common/Smallstep.v
@@ -30,6 +30,7 @@ Require Import Globalenvs.
 Require Import Integers.
 Require Import Tags.
 Require Import Values.
+Require Import Ctypes.
 
 Set Implicit Arguments.
 
@@ -52,57 +53,57 @@ Module Smallstep (Ptr: Pointer) (Pol: Policy)
         captures the observable events possibly generated during the
         transition. *)
 
-    Variable step: genv -> state -> trace -> state -> Prop.
+    Variable step: genv -> composite_env -> state -> trace -> state -> Prop.
 
     (** No transitions: stuck state *)
 
-    Definition nostep (ge: genv) (s: state) : Prop :=
-      forall t s', ~(step ge s t s').
+    Definition nostep (ge: genv) (ce: composite_env) (s: state) : Prop :=
+      forall t s', ~(step ge ce s t s').
 
     (** Zero, one or several transitions.  Also known as Kleene closure,
         or reflexive transitive closure. *)
 
-    Inductive star (ge: genv): state -> trace -> state -> Prop :=
+    Inductive star (ge: genv) (ce: composite_env): state -> trace -> state -> Prop :=
     | star_refl: forall s,
-        star ge s E0 s
+        star ge ce s E0 s
     | star_step: forall s1 t1 s2 t2 s3 t,
-        step ge s1 t1 s2 -> star ge s2 t2 s3 -> t = t1 ** t2 ->
-        star ge s1 t s3.
+        step ge ce s1 t1 s2 -> star ge ce s2 t2 s3 -> t = t1 ** t2 ->
+        star ge ce s1 t s3.
 
     Lemma star_one:
-      forall ge s1 t s2, step ge s1 t s2 -> star ge s1 t s2.
+      forall ge ce s1 t s2, step ge ce s1 t s2 -> star ge ce s1 t s2.
     Proof.
       intros. eapply star_step; eauto. apply star_refl. traceEq.
     Qed.
 
     Lemma star_two:
-      forall ge s1 t1 s2 t2 s3 t,
-        step ge s1 t1 s2 -> step ge s2 t2 s3 -> t = t1 ** t2 ->
-        star ge s1 t s3.
+      forall ge ce s1 t1 s2 t2 s3 t,
+        step ge ce s1 t1 s2 -> step ge ce s2 t2 s3 -> t = t1 ** t2 ->
+        star ge ce s1 t s3.
     Proof.
       intros. eapply star_step; eauto. apply star_one; auto.
     Qed.
     
     Lemma star_three:
-      forall ge s1 t1 s2 t2 s3 t3 s4 t,
-        step ge s1 t1 s2 -> step ge s2 t2 s3 -> step ge s3 t3 s4 -> t = t1 ** t2 ** t3 ->
-        star ge s1 t s4.
+      forall ge ce s1 t1 s2 t2 s3 t3 s4 t,
+        step ge ce s1 t1 s2 -> step ge ce s2 t2 s3 -> step ge ce s3 t3 s4 -> t = t1 ** t2 ** t3 ->
+        star ge ce s1 t s4.
     Proof.
       intros. eapply star_step; eauto. eapply star_two; eauto.
     Qed.
 
     Lemma star_four:
-      forall ge s1 t1 s2 t2 s3 t3 s4 t4 s5 t,
-        step ge s1 t1 s2 -> step ge s2 t2 s3 ->
-        step ge s3 t3 s4 -> step ge s4 t4 s5 -> t = t1 ** t2 ** t3 ** t4 ->
-        star ge s1 t s5.
+      forall ge ce s1 t1 s2 t2 s3 t3 s4 t4 s5 t,
+        step ge ce s1 t1 s2 -> step ge ce s2 t2 s3 ->
+        step ge ce s3 t3 s4 -> step ge ce s4 t4 s5 -> t = t1 ** t2 ** t3 ** t4 ->
+        star ge ce s1 t s5.
     Proof.
       intros. eapply star_step; eauto. eapply star_three; eauto.
     Qed.
 
     Lemma star_trans:
-      forall ge s1 t1 s2, star ge s1 t1 s2 ->
-                          forall t2 s3 t, star ge s2 t2 s3 -> t = t1 ** t2 -> star ge s1 t s3.
+      forall ge ce s1 t1 s2, star ge ce s1 t1 s2 ->
+                          forall t2 s3 t, star ge ce s2 t2 s3 -> t = t1 ** t2 -> star ge ce s1 t s3.
     Proof.
       induction 1; intros.
       - rewrite H0. simpl. auto.
@@ -110,27 +111,27 @@ Module Smallstep (Ptr: Pointer) (Pol: Policy)
     Qed.
 
     Lemma star_left:
-      forall ge s1 t1 s2 t2 s3 t,
-        step ge s1 t1 s2 -> star ge s2 t2 s3 -> t = t1 ** t2 ->
-        star ge s1 t s3.
+      forall ge ce s1 t1 s2 t2 s3 t,
+        step ge ce s1 t1 s2 -> star ge ce s2 t2 s3 -> t = t1 ** t2 ->
+        star ge ce s1 t s3.
     Proof star_step.
 
     Lemma star_right:
-      forall ge s1 t1 s2 t2 s3 t,
-        star ge s1 t1 s2 -> step ge s2 t2 s3 -> t = t1 ** t2 ->
-        star ge s1 t s3.
+      forall ge ce s1 t1 s2 t2 s3 t,
+        star ge ce s1 t1 s2 -> step ge ce s2 t2 s3 -> t = t1 ** t2 ->
+        star ge ce s1 t s3.
     Proof.
       intros. eapply star_trans. eauto. apply star_one. eauto. auto.
     Qed.
 
     Lemma star_E0_ind:
-      forall ge (P: state -> state -> Prop),
+      forall ge ce (P: state -> state -> Prop),
         (forall s, P s s) ->
-        (forall s1 s2 s3, step ge s1 E0 s2 -> P s2 s3 -> P s1 s3) ->
-        forall s1 s2, star ge s1 E0 s2 -> P s1 s2.
+        (forall s1 s2 s3, step ge ce s1 E0 s2 -> P s2 s3 -> P s1 s3) ->
+        forall s1 s2, star ge ce s1 E0 s2 -> P s1 s2.
     Proof.
-      intros ge P BASE REC.
-      assert (forall s1 t s2, star ge s1 t s2 -> t = E0 -> P s1 s2).
+      intros ge ce P BASE REC.
+      assert (forall s1 t s2, star ge ce s1 t s2 -> t = E0 -> P s1 s2).
       induction 1; intros; subst.
       auto.
       destruct (Eapp_E0_inv _ _ H2). subst. eauto.
@@ -139,54 +140,54 @@ Module Smallstep (Ptr: Pointer) (Pol: Policy)
     
     (** One or several transitions.  Also known as the transitive closure. *)
 
-    Inductive plus (ge: genv): state -> trace -> state -> Prop :=
+    Inductive plus (ge: genv) (ce: composite_env) : state -> trace -> state -> Prop :=
     | plus_left: forall s1 t1 s2 t2 s3 t,
-        step ge s1 t1 s2 -> star ge s2 t2 s3 -> t = t1 ** t2 ->
-        plus ge s1 t s3.
+        step ge ce s1 t1 s2 -> star ge ce s2 t2 s3 -> t = t1 ** t2 ->
+        plus ge ce s1 t s3.
 
     Lemma plus_one:
-      forall ge s1 t s2,
-        step ge s1 t s2 -> plus ge s1 t s2.
+      forall ge ce s1 t s2,
+        step ge ce s1 t s2 -> plus ge ce s1 t s2.
     Proof.
       intros. econstructor; eauto. apply star_refl. traceEq.
     Qed.
 
     Lemma plus_two:
-      forall ge s1 t1 s2 t2 s3 t,
-        step ge s1 t1 s2 -> step ge s2 t2 s3 -> t = t1 ** t2 ->
-        plus ge s1 t s3.
+      forall ge ce s1 t1 s2 t2 s3 t,
+        step ge ce s1 t1 s2 -> step ge ce s2 t2 s3 -> t = t1 ** t2 ->
+        plus ge ce s1 t s3.
     Proof.
       intros. eapply plus_left; eauto. apply star_one; auto.
     Qed.
 
     Lemma plus_three:
-      forall ge s1 t1 s2 t2 s3 t3 s4 t,
-        step ge s1 t1 s2 -> step ge s2 t2 s3 -> step ge s3 t3 s4 -> t = t1 ** t2 ** t3 ->
-        plus ge s1 t s4.
+      forall ge ce s1 t1 s2 t2 s3 t3 s4 t,
+        step ge ce s1 t1 s2 -> step ge ce s2 t2 s3 -> step ge ce s3 t3 s4 -> t = t1 ** t2 ** t3 ->
+        plus ge ce s1 t s4.
     Proof.
       intros. eapply plus_left; eauto. eapply star_two; eauto.
     Qed.
 
     Lemma plus_four:
-      forall ge s1 t1 s2 t2 s3 t3 s4 t4 s5 t,
-        step ge s1 t1 s2 -> step ge s2 t2 s3 ->
-        step ge s3 t3 s4 -> step ge s4 t4 s5 -> t = t1 ** t2 ** t3 ** t4 ->
-        plus ge s1 t s5.
+      forall ge ce s1 t1 s2 t2 s3 t3 s4 t4 s5 t,
+        step ge ce s1 t1 s2 -> step ge ce s2 t2 s3 ->
+        step ge ce s3 t3 s4 -> step ge ce s4 t4 s5 -> t = t1 ** t2 ** t3 ** t4 ->
+        plus ge ce s1 t s5.
     Proof.
       intros. eapply plus_left; eauto. eapply star_three; eauto.
     Qed.
 
     Lemma plus_star:
-      forall ge s1 t s2, plus ge s1 t s2 -> star ge s1 t s2.
+      forall ge ce s1 t s2, plus ge ce s1 t s2 -> star ge ce s1 t s2.
     Proof.
       intros. inversion H; subst.
       eapply star_step; eauto.
     Qed.
 
     Lemma plus_right:
-      forall ge s1 t1 s2 t2 s3 t,
-        star ge s1 t1 s2 -> step ge s2 t2 s3 -> t = t1 ** t2 ->
-        plus ge s1 t s3.
+      forall ge ce s1 t1 s2 t2 s3 t,
+        star ge ce s1 t1 s2 -> step ge ce s2 t2 s3 -> t = t1 ** t2 ->
+        plus ge ce s1 t s3.
     Proof.
       intros. inversion H; subst. simpl. apply plus_one. auto.
       rewrite Eapp_assoc. eapply plus_left; eauto.
@@ -194,24 +195,24 @@ Module Smallstep (Ptr: Pointer) (Pol: Policy)
     Qed.
 
     Lemma plus_left':
-      forall ge s1 t1 s2 t2 s3 t,
-        step ge s1 t1 s2 -> plus ge s2 t2 s3 -> t = t1 ** t2 ->
-        plus ge s1 t s3.
+      forall ge ce s1 t1 s2 t2 s3 t,
+        step ge ce s1 t1 s2 -> plus ge ce s2 t2 s3 -> t = t1 ** t2 ->
+        plus ge ce s1 t s3.
     Proof.
       intros. eapply plus_left; eauto. apply plus_star; auto.
     Qed.
 
     Lemma plus_right':
-      forall ge s1 t1 s2 t2 s3 t,
-        plus ge s1 t1 s2 -> step ge s2 t2 s3 -> t = t1 ** t2 ->
-        plus ge s1 t s3.
+      forall ge ce s1 t1 s2 t2 s3 t,
+        plus ge ce s1 t1 s2 -> step ge ce s2 t2 s3 -> t = t1 ** t2 ->
+        plus ge ce s1 t s3.
     Proof.
       intros. eapply plus_right; eauto. apply plus_star; auto.
     Qed.
 
     Lemma plus_star_trans:
-      forall ge s1 t1 s2 t2 s3 t,
-        plus ge s1 t1 s2 -> star ge s2 t2 s3 -> t = t1 ** t2 -> plus ge s1 t s3.
+      forall ge ce s1 t1 s2 t2 s3 t,
+        plus ge ce s1 t1 s2 -> star ge ce s2 t2 s3 -> t = t1 ** t2 -> plus ge ce s1 t s3.
     Proof.
       intros. inversion H; subst.
       econstructor; eauto. eapply star_trans; eauto.
@@ -219,8 +220,8 @@ Module Smallstep (Ptr: Pointer) (Pol: Policy)
     Qed.
 
     Lemma star_plus_trans:
-      forall ge s1 t1 s2 t2 s3 t,
-        star ge s1 t1 s2 -> plus ge s2 t2 s3 -> t = t1 ** t2 -> plus ge s1 t s3.
+      forall ge ce s1 t1 s2 t2 s3 t,
+        star ge ce s1 t1 s2 -> plus ge ce s2 t2 s3 -> t = t1 ** t2 -> plus ge ce s1 t s3.
     Proof.
       intros. inversion H; subst.
       simpl; auto.
@@ -230,16 +231,16 @@ Module Smallstep (Ptr: Pointer) (Pol: Policy)
     Qed.
 
     Lemma plus_trans:
-      forall ge s1 t1 s2 t2 s3 t,
-        plus ge s1 t1 s2 -> plus ge s2 t2 s3 -> t = t1 ** t2 -> plus ge s1 t s3.
+      forall ge ce s1 t1 s2 t2 s3 t,
+        plus ge ce s1 t1 s2 -> plus ge ce s2 t2 s3 -> t = t1 ** t2 -> plus ge ce s1 t s3.
     Proof.
       intros. eapply plus_star_trans. eauto. apply plus_star. eauto. auto.
     Qed.
 
     Lemma plus_inv:
-      forall ge s1 t s2,
-        plus ge s1 t s2 ->
-        step ge s1 t s2 \/ exists s', exists t1, exists t2, step ge s1 t1 s' /\ plus ge s' t2 s2 /\ t = t1 ** t2.
+      forall ge ce s1 t s2,
+        plus ge ce s1 t s2 ->
+        step ge ce s1 t s2 \/ exists s', exists t1, exists t2, step ge ce s1 t1 s' /\ plus ge ce s' t2 s2 /\ t = t1 ** t2.
     Proof.
       intros. inversion H; subst. inversion H1; subst.
       left. rewrite E0_right. auto.
@@ -248,24 +249,24 @@ Module Smallstep (Ptr: Pointer) (Pol: Policy)
     Qed.
 
     Lemma star_inv:
-      forall ge s1 t s2,
-        star ge s1 t s2 ->
-        (s2 = s1 /\ t = E0) \/ plus ge s1 t s2.
+      forall ge ce s1 t s2,
+        star ge ce s1 t s2 ->
+        (s2 = s1 /\ t = E0) \/ plus ge ce s1 t s2.
     Proof.
       intros. inv H. left; auto. right; econstructor; eauto.
     Qed.
 
     Lemma plus_ind2:
-      forall ge (P: state -> trace -> state -> Prop),
-        (forall s1 t s2, step ge s1 t s2 -> P s1 t s2) ->
+      forall ge ce (P: state -> trace -> state -> Prop),
+        (forall s1 t s2, step ge ce s1 t s2 -> P s1 t s2) ->
         (forall s1 t1 s2 t2 s3 t,
-            step ge s1 t1 s2 -> plus ge s2 t2 s3 -> P s2 t2 s3 -> t = t1 ** t2 ->
+            step ge ce s1 t1 s2 -> plus ge ce s2 t2 s3 -> P s2 t2 s3 -> t = t1 ** t2 ->
             P s1 t s3) ->
-        forall s1 t s2, plus ge s1 t s2 -> P s1 t s2.
+        forall s1 t s2, plus ge ce s1 t s2 -> P s1 t s2.
     Proof.
-      intros ge P BASE IND.
-      assert (forall s1 t s2, star ge s1 t s2 ->
-                              forall s0 t0, step ge s0 t0 s1 ->
+      intros ge ce P BASE IND.
+      assert (forall s1 t s2, star ge ce s1 t s2 ->
+                              forall s0 t0, step ge ce s0 t0 s1 ->
                                             P s0 (t0 ** t) s2).
       induction 1; intros.
       rewrite E0_right. apply BASE; auto.
@@ -275,30 +276,30 @@ Module Smallstep (Ptr: Pointer) (Pol: Policy)
     Qed.
 
     Lemma plus_E0_ind:
-      forall ge (P: state -> state -> Prop),
-        (forall s1 s2 s3, step ge s1 E0 s2 -> star ge s2 E0 s3 -> P s1 s3) ->
-        forall s1 s2, plus ge s1 E0 s2 -> P s1 s2.
+      forall ge ce (P: state -> state -> Prop),
+        (forall s1 s2 s3, step ge ce s1 E0 s2 -> star ge ce s2 E0 s3 -> P s1 s3) ->
+        forall s1 s2, plus ge ce s1 E0 s2 -> P s1 s2.
     Proof.
       intros. inv H0. exploit Eapp_E0_inv; eauto. intros [A B]; subst. eauto.
     Qed.
 
     (** Counted sequences of transitions *)
     
-    Inductive starN (ge: genv): nat -> state -> trace -> state -> Prop :=
+    Inductive starN (ge: genv) (ce: composite_env) : nat -> state -> trace -> state -> Prop :=
     | starN_refl: forall s,
-        starN ge O s E0 s
+        starN ge ce O s E0 s
     | starN_step: forall n s t t1 s' t2 s'',
-        step ge s t1 s' -> starN ge n s' t2 s'' -> t = t1 ** t2 ->
-        starN ge (S n) s t s''.
+        step ge ce s t1 s' -> starN ge ce n s' t2 s'' -> t = t1 ** t2 ->
+        starN ge ce (S n) s t s''.
     
     Remark starN_star:
-      forall ge n s t s', starN ge n s t s' -> star ge s t s'.
+      forall ge ce n s t s', starN ge ce n s t s' -> star ge ce s t s'.
     Proof.
       induction 1; econstructor; eauto.
     Qed.
 
     Remark star_starN:
-      forall ge s t s', star ge s t s' -> exists n, starN ge n s t s'.
+      forall ge ce s t s', star ge ce s t s' -> exists n, starN ge ce n s t s'.
     Proof.
       induction 1.
       exists O; constructor.
@@ -307,15 +308,15 @@ Module Smallstep (Ptr: Pointer) (Pol: Policy)
 
     (** Infinitely many transitions *)
     
-    CoInductive forever (ge: genv): state -> traceinf -> Prop :=
+    CoInductive forever (ge: genv) (ce: composite_env) : state -> traceinf -> Prop :=
     | forever_intro: forall s1 t s2 T,
-        step ge s1 t s2 -> forever ge s2 T ->
-        forever ge s1 (t *** T).
+        step ge ce s1 t s2 -> forever ge ce s2 T ->
+        forever ge ce s1 (t *** T).
     
     Lemma star_forever:
-      forall ge s1 t s2, star ge s1 t s2 ->
-                         forall T, forever ge s2 T ->
-                                   forever ge s1 (t *** T).
+      forall ge ce s1 t s2, star ge ce s1 t s2 ->
+                         forall T, forever ge ce s2 T ->
+                                   forever ge ce s1 (t *** T).
     Proof.
       induction 1; intros. simpl. auto.
       subst t0. rewrite Eappinf_assoc.
@@ -328,28 +329,28 @@ Module Smallstep (Ptr: Pointer) (Pol: Policy)
     Variable A: Type.
     Variable order: A -> A -> Prop.
 
-    CoInductive forever_N (ge: genv) : A -> state -> traceinf -> Prop :=
+    CoInductive forever_N (ge: genv) (ce: composite_env) : A -> state -> traceinf -> Prop :=
     | forever_N_star: forall s1 t s2 a1 a2 T1 T2,
-        star ge s1 t s2 ->
+        star ge ce s1 t s2 ->
         order a2 a1 ->
-        forever_N ge a2 s2 T2 ->
+        forever_N ge ce a2 s2 T2 ->
         T1 = t *** T2 ->
-        forever_N ge a1 s1 T1
+        forever_N ge ce a1 s1 T1
     | forever_N_plus: forall s1 t s2 a1 a2 T1 T2,
-        plus ge s1 t s2 ->
-        forever_N ge a2 s2 T2 ->
+        plus ge ce s1 t s2 ->
+        forever_N ge ce a2 s2 T2 ->
         T1 = t *** T2 ->
-        forever_N ge a1 s1 T1.
+        forever_N ge ce a1 s1 T1.
 
     Hypothesis order_wf: well_founded order.
 
     Lemma forever_N_inv:
-      forall ge a s T,
-        forever_N ge a s T ->
+      forall ge ce a s T,
+        forever_N ge ce a s T ->
         exists t, exists s', exists a', exists T',
-          step ge s t s' /\ forever_N ge a' s' T' /\ T = t *** T'.
+          step ge ce s t s' /\ forever_N ge ce a' s' T' /\ T = t *** T'.
     Proof.
-      intros ge a0. pattern a0. apply (well_founded_ind order_wf).
+      intros ge ce a0. pattern a0. apply (well_founded_ind order_wf).
       intros. inv H0.
       (* star case *)
       inv H1.
@@ -369,7 +370,7 @@ Module Smallstep (Ptr: Pointer) (Pol: Policy)
     Qed.
 
     Lemma forever_N_forever:
-      forall ge a s T, forever_N ge a s T -> forever ge s T.
+      forall ge ce a s T, forever_N ge ce a s T -> forever ge ce s T.
     Proof.
       cofix COINDHYP; intros.
       destruct (forever_N_inv H) as [t [s' [a' [T' [P [Q R]]]]]].
@@ -379,18 +380,18 @@ Module Smallstep (Ptr: Pointer) (Pol: Policy)
     
     (** Yet another alternative definition of [forever]. *)
 
-    CoInductive forever_plus (ge: genv) : state -> traceinf -> Prop :=
+    CoInductive forever_plus (ge: genv) (ce: composite_env) : state -> traceinf -> Prop :=
     | forever_plus_intro: forall s1 t s2 T1 T2,
-        plus ge s1 t s2 ->
-        forever_plus ge s2 T2 ->
+        plus ge ce s1 t s2 ->
+        forever_plus ge ce s2 T2 ->
         T1 = t *** T2 ->
-        forever_plus ge s1 T1.
+        forever_plus ge ce s1 T1.
     
     Lemma forever_plus_inv:
-      forall ge s T,
-        forever_plus ge s T ->
+      forall ge ce s T,
+        forever_plus ge ce s T ->
         exists s', exists t, exists T',
-          step ge s t s' /\ forever_plus ge s' T' /\ T = t *** T'.
+          step ge ce s t s' /\ forever_plus ge ce s' T' /\ T = t *** T'.
     Proof.
       intros. inv H. inv H0. exists s0; exists t1; exists (t2 *** T2).
       split. auto.
@@ -400,7 +401,7 @@ Module Smallstep (Ptr: Pointer) (Pol: Policy)
     Qed.
 
     Lemma forever_plus_forever:
-      forall ge s T, forever_plus ge s T -> forever ge s T.
+      forall ge ce s T, forever_plus ge ce s T -> forever ge ce s T.
     Proof.
       cofix COINDHYP; intros.
       destruct (forever_plus_inv H) as [s' [t [T' [P [Q R]]]]].
@@ -409,31 +410,31 @@ Module Smallstep (Ptr: Pointer) (Pol: Policy)
     
     (** Infinitely many silent transitions *)
     
-    CoInductive forever_silent (ge: genv): state -> Prop :=
+    CoInductive forever_silent (ge: genv) (ce: composite_env): state -> Prop :=
     | forever_silent_intro: forall s1 s2,
-        step ge s1 E0 s2 -> forever_silent ge s2 ->
-        forever_silent ge s1.
+        step ge ce s1 E0 s2 -> forever_silent ge ce s2 ->
+        forever_silent ge ce s1.
     
     (** An alternate definition. *)
     
-    CoInductive forever_silent_N (ge: genv) : A -> state -> Prop :=
+    CoInductive forever_silent_N (ge: genv) (ce: composite_env) : A -> state -> Prop :=
     | forever_silent_N_star: forall s1 s2 a1 a2,
-        star ge s1 E0 s2 ->
+        star ge ce s1 E0 s2 ->
         order a2 a1 ->
-        forever_silent_N ge a2 s2 ->
-        forever_silent_N ge a1 s1
+        forever_silent_N ge ce a2 s2 ->
+        forever_silent_N ge ce a1 s1
     | forever_silent_N_plus: forall s1 s2 a1 a2,
-        plus ge s1 E0 s2 ->
-        forever_silent_N ge a2 s2 ->
-        forever_silent_N ge a1 s1.
+        plus ge ce s1 E0 s2 ->
+        forever_silent_N ge ce a2 s2 ->
+        forever_silent_N ge ce a1 s1.
 
     Lemma forever_silent_N_inv:
-      forall ge a s,
-        forever_silent_N ge a s ->
+      forall ge ce a s,
+        forever_silent_N ge ce a s ->
         exists s', exists a',
-          step ge s E0 s' /\ forever_silent_N ge a' s'.
+          step ge ce s E0 s' /\ forever_silent_N ge ce a' s'.
     Proof.
-      intros ge a0. pattern a0. apply (well_founded_ind order_wf).
+      intros ge ce a0. pattern a0. apply (well_founded_ind order_wf).
       intros. inv H0.
       (* star case *)
       inv H1.
@@ -451,7 +452,7 @@ Module Smallstep (Ptr: Pointer) (Pol: Policy)
     Qed.
     
     Lemma forever_silent_N_forever:
-      forall ge a s, forever_silent_N ge a s -> forever_silent ge s.
+      forall ge ce a s, forever_silent_N ge ce a s -> forever_silent ge ce s.
     Proof.
       cofix COINDHYP; intros.
       destruct (forever_silent_N_inv H) as [s' [a' [P Q]]].
@@ -461,15 +462,15 @@ Module Smallstep (Ptr: Pointer) (Pol: Policy)
     
     (** Infinitely many non-silent transitions *)
     
-    CoInductive forever_reactive (ge: genv): state -> traceinf -> Prop :=
+    CoInductive forever_reactive (ge: genv) (ce: composite_env): state -> traceinf -> Prop :=
     | forever_reactive_intro: forall s1 s2 t T,
-        star ge s1 t s2 -> t <> E0 -> forever_reactive ge s2 T ->
-        forever_reactive ge s1 (t *** T).
+        star ge ce s1 t s2 -> t <> E0 -> forever_reactive ge ce s2 T ->
+        forever_reactive ge ce s1 (t *** T).
     
     Lemma star_forever_reactive:
-      forall ge s1 t s2 T,
-        star ge s1 t s2 -> forever_reactive ge s2 T ->
-        forever_reactive ge s1 (t *** T).
+      forall ge ce s1 t s2 T,
+        star ge ce s1 t s2 -> forever_reactive ge ce s2 T ->
+        forever_reactive ge ce s1 (t *** T).
     Proof.
       intros. inv H0. rewrite <- Eappinf_assoc. econstructor.
       eapply star_trans; eauto.
@@ -488,26 +489,29 @@ Module Smallstep (Ptr: Pointer) (Pol: Policy)
         state: Type;
         funtype: Type;
         vartype: Type;                            
-        step : Genv.t funtype vartype -> state -> trace -> state -> Prop;
+        step : Genv.t funtype vartype -> composite_env -> state -> trace -> state -> Prop;
         initial_state: state -> Prop;
         final_state: state -> int -> Prop;
         globalenv: Genv.t funtype vartype;
+        ce: composite_env;
       }.
 
   (** The form used in earlier CompCert versions, for backward compatibility. *)
 
   Definition Semantics {state funtype vartype: Type}
-             (step: Genv.t funtype vartype -> state -> trace -> state -> Prop)
+             (step: Genv.t funtype vartype -> composite_env -> state -> trace -> state -> Prop)
              (initial_state: state -> Prop)
              (final_state: state -> int -> Prop)
-             (globalenv: Genv.t funtype vartype) :=
+             (globalenv: Genv.t funtype vartype)
+             (ce: composite_env) :=
     {| state := state;
       funtype := funtype;
       vartype := vartype;
       step := step;
       initial_state := initial_state;
       final_state := final_state;
-      globalenv := globalenv |}.
+      globalenv := globalenv;
+      ce := ce |}.
   
   (** Handy notations. *)
 
@@ -522,305 +526,19 @@ Module Smallstep (Ptr: Pointer) (Pol: Policy)
 
 End Smallstep.
 
-(** * Forward simulations between two transition semantics. *)
-
-(** The general form of a forward simulation. *)
-
-Module FSIM (Ptr1: Pointer) (Pol1: Policy)
-       (M1: Memory Ptr1 Pol1) (A1: Allocator Ptr1 Pol1 M1)
-       (Ptr2: Pointer) (Pol2: Policy)
-       (M2: Memory Ptr2 Pol2) (A2: Allocator Ptr2 Pol2 M2).
-  Module S1 := Smallstep Ptr1 Pol1 M1 A1.
-  Module E1 := S1.Events.
-  Module GV1 := E1.Genv.
-  Module S2 := Smallstep Ptr2 Pol2 M2 A2.
-  Module E2 := S2.Events.
-  Module GV2 := E2.Genv.
-  
-  Inductive eventval_match: E1.eventval -> E2.eventval -> Prop :=
-  | MEVint: forall i,
-      eventval_match (E1.EVint i) (E2.EVint i)
-  | MEVlong: forall i,
-      eventval_match (E1.EVlong i) (E2.EVlong i)
-  | MEVfloat: forall f,
-      eventval_match (E1.EVfloat f) (E2.EVfloat f)
-  | MEVsingle: forall f,
-      eventval_match (E1.EVfloat f) (E2.EVfloat f)
-  | MEVptr_global: forall id p1 p2,
-      (Ptr1.concretize p1) = (Ptr2.concretize p2) ->
-      eventval_match (E1.EVptr_global id p1) (E2.EVptr_global id p2)
-  | MEVptr_fun: forall id,
-      eventval_match (E1.EVptr_fun id) (E2.EVptr_fun id)      
-  .
-
-  Inductive ev_list_match: list E1.eventval -> list E2.eventval -> Prop :=
-  | MEVLnil: ev_list_match nil nil
-  | MEVLcons: forall ev1 ev2 evs1 evs2,
-      eventval_match ev1 ev2 ->
-      ev_list_match evs1 evs2 ->
-      ev_list_match (ev1::evs1) (ev2::evs2)
-  .
-  
-  Inductive event_match: E1.event -> E2.event -> Prop :=
-  | MEvent_syscall: forall s evs1 evs2 ev1 ev2,
-      ev_list_match evs1 evs2 ->
-      eventval_match ev1 ev2 ->
-      event_match (E1.Event_syscall s evs1 ev1) (E2.Event_syscall s evs2 ev2)
-  | MEvent_vload: forall chunk id p1 p2 ev1 ev2,
-      (Ptr1.concretize p1) = (Ptr2.concretize p2) ->
-      eventval_match ev1 ev2 ->
-      event_match (E1.Event_vload chunk id p1 ev1) (E2.Event_vload chunk id p2 ev2)
-  | MEvent_vstore: forall chunk id p1 p2 ev1 ev2,
-      (Ptr1.concretize p1) = (Ptr2.concretize p2) ->
-      eventval_match ev1 ev2 ->
-      event_match (E1.Event_vstore chunk id p1 ev1) (E2.Event_vstore chunk id p2 ev2)
-  | MEvent_annot: forall s evs1 evs2,
-      ev_list_match evs1 evs2 ->
-      event_match (E1.Event_annot s evs1) (E2.Event_annot s evs2).
-
-  Inductive match_traces : E1.trace -> E2.trace -> Prop :=
-  | MTnil: match_traces nil nil
-  | MTcons: forall e1 e2 t1 t2,
-      event_match e1 e2 ->
-      match_traces t1 t2 ->
-      match_traces (e1::t1) (e2::t2).
-
-  CoInductive traceinf_match : E1.traceinf -> E2.traceinf -> Prop :=
-  | MEconsinf: forall e1 e2 t1 t2,
-      event_match e1 e2 ->
-      traceinf_match t1 t2 ->
-      traceinf_match (E1.Econsinf e1 t1) (E2.Econsinf e2 t2).
-
-  (** Handy notations, now for both! *)
-
-  Notation " 'S1.Step' L " := (S1.step L (S1.globalenv L)) (at level 1) : smallstep_scope.
-  Notation " 'S1.Star' L " := (S1.star (S1.step L) (S1.globalenv L)) (at level 1) : smallstep_scope.
-  Notation " 'S1.Plus' L " := (S1.plus (S1.step L) (S1.globalenv L)) (at level 1) : smallstep_scope.
-  Notation " 'S1.Forever_silent' L " := (S1.forever_silent (S1.step L) (S1.globalenv L)) (at level 1) : smallstep_scope.
-  Notation " 'S1.Forever_reactive' L " := (S1.forever_reactive (S1.step L) (S1.globalenv L)) (at level 1) : smallstep_scope.
-  Notation " 'S1.Nostep' L " := (S1.nostep (S1.step L) (S1.globalenv L)) (at level 1) : smallstep_scope.
-
-  Notation " 'S2.Step' L " := (S2.step L (S2.globalenv L)) (at level 1) : smallstep_scope.
-  Notation " 'S2.Star' L " := (S2.star (S2.step L) (S2.globalenv L)) (at level 1) : smallstep_scope.
-  Notation " 'S2.Plus' L " := (S2.plus (S2.step L) (S2.globalenv L)) (at level 1) : smallstep_scope.
-  Notation " 'S2.Forever_silent' L " := (S2.forever_silent (S2.step L) (S2.globalenv L)) (at level 1) : smallstep_scope.
-  Notation " 'S2.Forever_reactive' L " := (S2.forever_reactive (S2.step L) (S2.globalenv L)) (at level 1) : smallstep_scope.
-  Notation " 'S2.Nostep' L " := (S2.nostep (S2.step L) (S2.globalenv L)) (at level 1) : smallstep_scope.
-  
-  Open Scope smallstep_scope.
-  
-  Record fsim_properties (L1: S1.semantics) (L2: S2.semantics) (index: Type)
-         (order: index -> index -> Prop)
-         (match_states: index -> S1.state L1 -> S2.state L2 -> Prop) : Prop := {
-      fsim_order_wf: well_founded order;
-      fsim_match_initial_states:
-      forall s1, S1.initial_state L1 s1 ->
-                 exists i, exists s2, S2.initial_state L2 s2 /\ match_states i s1 s2;
-      fsim_match_final_states:
-      forall i s1 s2 r,
-        match_states i s1 s2 -> S1.final_state L1 s1 r -> S2.final_state L2 s2 r;
-      fsim_simulation:
-      forall s1 t1 s1', S1.Step L1 s1 t1 s1' ->
-                       forall i s2, match_states i s1 s2 ->
-                                    exists i', exists s2', exists t2,
-                                      (S2.Plus L2 s2 t2 s2' \/
-                                         (S2.Star L2 s2 t2 s2' /\ order i' i))
-                                      /\ match_states i' s1' s2' /\ match_traces t1 t2;
-      fsim_public_preserved:
-      forall id, GV2.public_symbol L2.(S2.globalenv) id = GV1.public_symbol L1.(S1.globalenv) id
-    }.
-
-Arguments fsim_properties: clear implicits.
-
-Inductive forward_simulation (L1: S1.semantics) (L2: S2.semantics) : Prop :=
-  Forward_simulation (index: Type)
-                     (order: index -> index -> Prop)
-                     (match_states: index -> S1.state L1 -> S2.state L2 -> Prop)
-                     (props: fsim_properties L1 L2 index order match_states).
-
-Arguments Forward_simulation {L1 L2 index} order match_states props.
-
-(** An alternate form of the simulation diagram *)
-
-Lemma fsim_simulation':
-  forall L1 L2 index order match_states, fsim_properties L1 L2 index order match_states ->
-  forall i s1 t1 s1', S1.Step L1 s1 t1 s1' ->
-  forall s2, match_states i s1 s2 ->
-  (exists i', exists s2', exists t2, S2.Plus L2 s2 t2 s2' /\ match_states i' s1' s2' /\ match_traces t1 t2)
-  \/ (exists i', order i' i /\ t1 = E1.E0 /\ match_states i' s1' s2).
-Proof.
-  intros. exploit fsim_simulation; eauto.
-  intros [i' [s2' [t2 [A [B C]]]]]. intuition.
-  left; exists i'; exists s2'; exists t2; auto.
-  inv H3. inv C.
-  right; exists i'; auto.
-  left; exists i'; exists s2'; exists (S2.Events.Eapp t0 t3); split; auto. econstructor; eauto.
-Qed.
-
-(** ** Forward simulation diagrams. *)
-
-(** Various simulation diagrams that imply forward simulation *)
-
-Section FORWARD_SIMU_DIAGRAMS.
-
-  Variable L1: S1.semantics.
-  Variable L2: S2.semantics.
-  
-  Hypothesis public_preserved:
-    forall id, GV2.public_symbol (S2.globalenv L2) id = GV1.public_symbol (S1.globalenv L1) id.
-
-  Variable match_states: S1.state L1 -> S2.state L2 -> Prop.
-
-  Hypothesis match_initial_states:
-    forall s1, S1.initial_state L1 s1 ->
-               exists s2, S2.initial_state L2 s2 /\ match_states s1 s2.
-
-  Hypothesis match_final_states:
-    forall s1 s2 r,
-      match_states s1 s2 ->
-      S1.final_state L1 s1 r ->
-      S2.final_state L2 s2 r.
-
-  (** Simulation when one transition in the first program
-      corresponds to zero, one or several transitions in the second program.
-      However, there is no stuttering: infinitely many transitions
-      in the source program must correspond to infinitely many
-      transitions in the second program. *)
-
-  Section SIMULATION_STAR_WF.
-
-    (** [order] is a well-founded ordering associated with states
-        of the first semantics.  Stuttering steps must correspond
-        to states that decrease w.r.t. [order]. *)
-
-    Variable order: S1.state L1 -> S1.state L1 -> Prop.
-    Hypothesis order_wf: well_founded order.
-
-    Hypothesis simulation:
-      forall s1 t1 s1', S1.Step L1 s1 t1 s1' ->
-                       forall s2, match_states s1 s2 ->
-                                  exists s2' t2,
-                                    (S2.Plus L2 s2 t2 s2' \/ (S2.Star L2 s2 t2 s2' /\ order s1' s1))
-                                    /\ match_states s1' s2' /\ match_traces t1 t2.
-
-    Lemma forward_simulation_star_wf: forward_simulation L1 L2.
-    Proof.
-      apply Forward_simulation with order (fun idx s1 s2 => idx = s1 /\ match_states s1 s2);
-        constructor.
-      - auto.
-      - intros. exploit match_initial_states; eauto. intros [s2 [A B]].
-        exists s1; exists s2; auto.
-      - intros. destruct H. eapply match_final_states; eauto.
-      - intros. destruct H0. subst i. exploit simulation; eauto. intros [s2' [t2 [A [B C]]]].
-        exists s1'; exists s2'; exists t2; intuition auto.
-      - auto.
-    Qed.
-
-  End SIMULATION_STAR_WF.
-
-  Section SIMULATION_STAR.
-
-    (** We now consider the case where we have a nonnegative integer measure
-        associated with states of the first semantics.  It must decrease when we take
-        a stuttering step. *)
-
-    Variable measure: S1.state L1 -> nat.
-
-    Hypothesis simulation:
-      forall s1 t1 s1', S1.Step L1 s1 t1 s1' ->
-                       forall s2, match_states s1 s2 ->
-                                  (exists s2', exists t2, S2.Plus L2 s2 t2 s2' /\ match_states s1' s2' /\ match_traces t1 t2)
-                                  \/ (measure s1' < measure s1 /\ t1 = E1.E0 /\ match_states s1' s2)%nat.
-
-    Lemma forward_simulation_star: forward_simulation L1 L2.
-    Proof.
-      apply forward_simulation_star_wf with (ltof _ measure).
-      apply well_founded_ltof.
-      intros. exploit simulation; eauto. intros [[s2' [t2 [A B]]] | [A [B C]]].
-      exists s2', t2; auto.
-      exists s2, E2.E0; split. right; split. constructor. rewrite B. apply star_refl. auto. auto.
-    Qed.
-
-  End SIMULATION_STAR.
-
-  (** Simulation when one transition in the first program corresponds
-      to one or several transitions in the second program. *)
-
-  Section SIMULATION_PLUS.
-
-    Hypothesis simulation:
-      forall s1 t s1', S1.Step L1 s1 t s1' ->
-                       forall s2, match_states s1 s2 ->
-                                  exists s2', S2.Plus L2 s2 t s2' /\ match_states s1' s2'.
-
-    Lemma forward_simulation_plus: forward_simulation L1 L2.
-    Proof.
-      apply forward_simulation_star with (measure := fun _ => O).
-      intros. exploit simulation; eauto.
-    Qed.
-
-  End SIMULATION_PLUS.
-*)
-  (** Lock-step simulation: each transition in the first semantics
-      corresponds to exactly one transition in the second semantics. *)
-  
-  Section SIMULATION_STEP.
-
-    Hypothesis simulation:
-      forall s1 t1 s1', S1.Step L1 s1 t1 s1' ->
-                       forall s2, match_states s1 s2 ->
-                                  exists s2' t2, S2.Step L2 s2 t2 s2' /\ match_states s1' s2'.
-
-    Lemma forward_simulation_step: forward_simulation L1 L2.
-    Proof.
-      apply forward_simulation_plus.
-      intros. exploit simulation; eauto. intros [s2' [A B]].
-      exists s2'; split; auto. apply plus_one; auto.
-    Qed.
-
-  End SIMULATION_STEP.
-
-  (** Simulation when one transition in the first program
-      corresponds to zero or one transitions in the second program.
-      However, there is no stuttering: infinitely many transitions
-      in the source program must correspond to infinitely many
-      transitions in the second program. *)
-
-  Section SIMULATION_OPT.
-
-    Variable measure: S1.state L1 -> nat.
-
-    Hypothesis simulation:
-      forall s1 t s1', S1.Step L1 s1 t s1' ->
-                       forall s2, match_states s1 s2 ->
-                                  (exists s2', Step L2 s2 t s2' /\ match_states s1' s2')
-                                  \/ (measure s1' < measure s1 /\ t = E0 /\ match_states s1' s2)%nat.
-
-    Lemma forward_simulation_opt: forward_simulation L1 L2.
-    Proof.
-      apply forward_simulation_star with measure.
-      intros. exploit simulation; eauto. intros [[s2' [A B]] | [A [B C]]].
-      left; exists s2'; split; auto. apply plus_one; auto.
-      right; auto.
-    Qed.
-
-  End SIMULATION_OPT.
-
-End FORWARD_SIMU_DIAGRAMS.
-
 (** ** Forward simulation of transition sequences *)
 
-Section SIMULATION_SEQUENCES.
+(*Section SIMULATION_SEQUENCES.
 
 Context L1 L2 index order match_states (S: fsim_properties L1 L2 index order match_states).
 
 Lemma simulation_star:
-  forall s1 t s1', Star L1 s1 t s1' ->
+  forall s1 t1 s1', S1.Star L1 s1 t1 s1' ->
   forall i s2, match_states i s1 s2 ->
-  exists i', exists s2', S2.Star L2 s2 t s2' /\ match_states i' s1' s2'.
+  exists i', exists s2', exists t2, S2.Star L2 s2 t2 s2' /\ match_states i' s1' s2'.
 Proof.
   induction 1; intros.
-  exists i; exists s2; split; auto. apply star_refl.
+  exists i; exists s2; exists t2; split; auto. apply star_refl.
   exploit fsim_simulation; eauto. intros [i' [s2' [A B]]].
   exploit IHstar; eauto. intros [i'' [s2'' [C D]]].
   exists i''; exists s2''; split; auto. eapply star_trans; eauto.
@@ -877,11 +595,13 @@ Proof.
 Qed.
 
 End SIMULATION_SEQUENCES.
-
+*)
 (** ** Composing two forward simulations *)
 
-Lemma compose_forward_simulations:
-  forall L1 L2 L3, forward_simulation L1 L2 -> forward_simulation L2 L3 -> forward_simulation L1 L3.
+(*Lemma compose_forward_simulations:
+  forall L1 L2 L3, forward_simulation L1 L2 ->
+                   forward_simulation L2 L3 ->
+                   forward_simulation L1 L3.
 Proof.
   intros L1 L2 L3 S12 S23.
   destruct S12 as [index order match_states props].
