common/Simulation.v
@@ -1,0 +1,493 @@
+Require Import Relations.
+Require Import Wellfounded.
+Require Import Coqlib.
+Require Import Allocator.
+Require Import Memory.
+Require Import Events.
+Require Import Globalenvs.
+Require Import Integers.
+Require Import Tags.
+Require Import Values.
+Require Import Csem.
+Require Import Csyntax.
+Require Import AST Ctypes.
+
+Module ProgEquiv (Ptr1: Pointer) (Pol1: Policy)
+       (M1: Memory Ptr1 Pol1) (A1: Allocator Ptr1 Pol1 M1)
+       (Ptr2: Pointer) (Pol2: Policy)
+       (M2: Memory Ptr2 Pol2) (A2: Allocator Ptr2 Pol2 M2).
+
+  Module Csem1 := Csem Ptr1 Pol1 M1 A1.
+  Module CS1 := Csem1.Csyntax.
+  Module Val1 := M1.MD.TLib.Switch.BI.BI1.BI0.Values.
+  Import Val1.
+  
+  Module Csem2 := Csem Ptr2 Pol2 M2 A2.
+  Module CS2 := Csem2.Csyntax.
+  Module Val2 := M2.MD.TLib.Switch.BI.BI1.BI0.Values.
+  Import Val2.
+  
+  Variable val_match : Val1.val -> Val2.val -> Prop.
+
+  Inductive expr_match : CS1.expr -> CS2.expr -> Prop :=
+  | MEvar : forall x ty,
+      expr_match (CS1.Evar x ty) (CS2.Evar x ty)
+  | MEconst : forall v1 v2 ty,
+      val_match v1 v2 ->
+      expr_match (CS1.Econst v1 ty) (CS2.Econst v2 ty)
+  | MEfield : forall l1 l2 f ty,
+      expr_match l1 l2 ->
+      expr_match (CS1.Efield l1 f ty) (CS2.Efield l2 f ty)
+  | MEvalof : forall l1 l2 ty,
+      expr_match l1 l2 ->
+      expr_match (CS1.Evalof l1 ty) (CS2.Evalof l2 ty)
+  | MEderef : forall r1 r2 ty,
+      expr_match r1 r2 ->
+      expr_match (CS1.Ederef r1 ty) (CS2.Ederef r2 ty)
+  | MEaddrof : forall l1 l2 ty,
+      expr_match l1 l2 ->
+      expr_match (CS1.Eaddrof l1 ty) (CS2.Eaddrof l2 ty)
+  | MEunop : forall op r1 r2 ty,
+      expr_match r1 r2 ->
+      expr_match (CS1.Eunop op r1 ty) (CS2.Eunop op r2 ty)
+  | MEbinop : forall op r1_1 r2_1 r1_2 r2_2 ty,
+      expr_match r1_1 r1_2 ->
+      expr_match r2_1 r2_2 ->
+      expr_match (CS1.Ebinop op r1_1 r2_1 ty) (CS2.Ebinop op r1_2 r2_2 ty)
+  | MEcast : forall r1 r2 ty,
+      expr_match r1 r2 ->
+      expr_match (CS1.Ecast r1 ty) (CS2.Ecast r2 ty)
+  | MEseqand : forall r1_1 r2_1 r1_2 r2_2 ty,
+      expr_match r1_1 r1_2 ->
+      expr_match r2_1 r2_2 ->
+      expr_match (CS1.Eseqand r1_1 r2_1 ty) (CS2.Eseqand r1_2 r2_2 ty)
+  | MEseqor : forall r1_1 r2_1 r1_2 r2_2 ty, 
+      expr_match r1_1 r1_2 ->
+      expr_match r2_1 r2_2 ->
+      expr_match (CS1.Eseqor r1_1 r2_1 ty) (CS2.Eseqor r1_2 r2_2 ty)
+  | MEcondition : forall r1_1 r2_1 r3_1 r1_2 r2_2 r3_2 ty,
+      expr_match r1_1 r1_2 ->
+      expr_match r2_1 r2_2 ->
+      expr_match r3_1 r3_2 ->
+      expr_match (CS1.Econdition r1_1 r2_1 r3_1 ty) (CS2.Econdition r1_2 r2_2 r3_2 ty)
+  | MEsizeof : forall ty' ty,  
+      expr_match (CS1.Esizeof ty' ty) (CS2.Esizeof ty' ty)
+  | MEalignof : forall ty' ty,       
+      expr_match (CS1.Ealignof ty' ty) (CS2.Ealignof ty' ty)
+  | MEassign : forall l1 l2 r1 r2 ty,
+      expr_match l1 l2 ->
+      expr_match r1 r2 ->
+      expr_match (CS1.Eassign l1 r1 ty) (CS2.Eassign l2 r2 ty)
+  | MEassignop : forall op l1 l2 r1 r2 tyres ty,
+      expr_match l1 l2 ->
+      expr_match r1 r2 ->
+      expr_match (CS1.Eassignop op l1 r1 tyres ty) (CS2.Eassignop op l2 r2 tyres ty)
+  | MEpostincr : forall l1 l2 ty,
+      expr_match l1 l2 ->
+      expr_match (CS1.Epostincr CS1.Cop.Incr l1 ty) (CS2.Epostincr CS2.Cop.Incr l2 ty)  | MEpostdecr : forall l1 l2 ty,
+      expr_match l1 l2 ->
+      expr_match (CS1.Epostincr CS1.Cop.Decr l1 ty) (CS2.Epostincr CS2.Cop.Decr l2 ty)
+  | MEcomma : forall r1_1 r2_1 r1_2 r2_2 ty,                  
+      expr_match r1_1 r1_2 ->
+      expr_match r2_1 r2_2 ->
+      expr_match (CS1.Ecomma r1_1 r2_1 ty) (CS2.Ecomma r1_2 r2_2 ty)
+  | MEcall : forall r1_1 r1_2 rargs1 rargs2 ty,
+      expr_match r1_1 r1_2 ->
+      exprlist_match rargs1 rargs2 ->
+      expr_match (CS1.Ecall r1_1 rargs1 ty) (CS2.Ecall r1_2 rargs2 ty)
+  | MEbuiltin : forall ef tyargs cc ty,
+      expr_match (CS1.Ebuiltin ef tyargs cc ty) (CS2.Ebuiltin ef tyargs cc ty)
+
+  with exprlist_match : CS1.exprlist -> CS2.exprlist -> Prop :=
+  | MEnil : exprlist_match CS1.Enil CS2.Enil
+  | MEcons : forall r1 r2 rl1 rl2,
+      expr_match r1 r2 ->
+      exprlist_match rl1 rl2 ->
+      exprlist_match (CS1.Econs r1 rl1) (CS2.Econs r2 rl2)
+  .
+
+  Inductive statement_match : CS1.statement -> CS2.statement -> Prop :=
+  | MSskip : statement_match CS1.Sskip CS2.Sskip
+  | MSSdo : forall e1 e2 l,
+      expr_match e1 e2 ->
+      statement_match (CS1.Sdo e1 l) (CS2.Sdo e2 l)
+  | MSsequence : forall s1_1 s2_1 s1_2 s2_2,
+        statement_match s1_1 s1_2 ->
+        statement_match s2_1 s2_2 ->
+        statement_match (CS1.Ssequence s1_1 s2_1) (CS2.Ssequence s1_2 s2_2)
+  | MSifthenelse : forall e1 e2 s1_1 s1_2 s2_1 s2_2 lb lc,
+      expr_match e1 e2 ->
+      statement_match s1_1 s1_2 ->
+      statement_match s2_1 s2_2 ->
+      statement_match (CS1.Sifthenelse e1 s1_1 s2_1 lb lc)
+                      (CS2.Sifthenelse e2 s1_2 s2_2 lb lc)
+  | MSwhile : forall e1 e2 s1 s2 lb lc,
+      expr_match e1 e2 ->
+      statement_match s1 s2 ->
+      statement_match (CS1.Swhile e1 s1 lb lc) (CS2.Swhile e2 s2 lb lc)
+  | MSdowhile : forall e1 e2 s1 s2 lb lc,
+      expr_match e1 e2 ->
+      statement_match s1 s2 ->
+      statement_match (CS1.Sdowhile e1 s1 lb lc) (CS2.Sdowhile e2 s2 lb lc)
+  | MSfor: forall s1_1 s1_2 e1 e2 s2_1 s2_2 s3_1 s3_2 lb lc,
+      statement_match s1_1 s1_2 ->
+      expr_match e1 e2 ->
+      statement_match s2_1 s2_2 ->
+      statement_match s3_1 s3_2 ->
+      statement_match (CS1.Sfor s1_1 e1 s2_1 s3_1 lb lc)
+                      (CS2.Sfor s1_2 e2 s2_2 s3_2 lb lc)                      
+  | MSbreak : forall l,
+      statement_match (CS1.Sbreak l) (CS2.Sbreak l)
+  | MScontinue : forall l,
+      statement_match (CS1.Scontinue l) (CS2.Scontinue l)
+  | MSreturn_Some : forall e1 e2 l,
+      expr_match e1 e2 ->
+      statement_match (CS1.Sreturn (Some e1) l) (CS2.Sreturn (Some e2) l)
+  | MSreturn_None : forall l,
+      statement_match (CS1.Sreturn None l) (CS2.Sreturn None l)     
+  | MSswitch : forall e1 e2 ls1 ls2 l,
+      expr_match e1 e2 ->
+      ls_match ls1 ls2 ->
+      statement_match (CS1.Sswitch e1 ls1 l) (CS2.Sswitch e2 ls2 l)
+  | MSlabel : forall l s1 s2,
+      statement_match s1 s2 ->
+      statement_match (CS1.Slabel l s1) (CS2.Slabel l s2)
+  | MSgoto : forall lb lc,
+      statement_match (CS1.Sgoto lb lc) (CS2.Sgoto lb lc)
+
+  with ls_match : CS1.labeled_statements -> CS2.labeled_statements -> Prop :=
+  | MLSnil: ls_match CS1.LSnil CS2.LSnil
+  | MLScons: forall z s1 s2 ls1 ls2,
+      statement_match s1 s2 ->
+      ls_match ls1 ls2 ->
+      ls_match (CS1.LScons z s1 ls1) (CS2.LScons z s2 ls2)
+  .
+  
+  Inductive fundef_match : CS1.fundef -> CS2.fundef -> Prop :=
+  | MFInternal : forall fn_ret fn_cc fn_params fn_vars fn_body1 fn_body2,
+      statement_match fn_body1 fn_body2 ->
+      fundef_match (Internal (CS1.mkfunction fn_ret fn_cc fn_params fn_vars fn_body1))
+                   (Internal (CS2.mkfunction fn_ret fn_cc fn_params fn_vars fn_body2))
+  | MFExternal : forall ef tyargs ty cc,
+      fundef_match (External ef tyargs ty cc) (External ef tyargs ty cc)
+  .
+
+  Inductive pd_match : list (ident*globdef CS1.fundef type) ->
+                       list (ident*globdef CS2.fundef type) ->
+                       Prop :=
+  | MPDnil : pd_match nil nil
+  | MPDcons_var : forall id gv pd1 pd2,
+      pd_match pd1 pd2 ->
+      pd_match ((id,Gvar gv)::pd1) ((id,Gvar gv)::pd2)
+  | MPDcons_fun : forall id fd1 fd2 pd1 pd2,
+      fundef_match fd1 fd2 ->
+      pd_match pd1 pd2 ->
+      pd_match ((id,Gfun fd1)::pd1) ((id,Gfun fd2)::pd2).
+  
+  Inductive prog_match : CS1.program -> CS2.program -> Prop :=
+  | MP : forall prog_defs1 prog_defs2 prog_public prog_main prog_types
+                prog_comp_env prog_comp_env_eq,
+      pd_match prog_defs1 prog_defs2 ->
+      prog_match (@Build_program CS1.function
+                                 prog_defs1 prog_public prog_main
+                                 prog_types prog_comp_env prog_comp_env_eq)
+                 (@Build_program CS2.function
+                                 prog_defs2 prog_public prog_main
+                                 prog_types prog_comp_env prog_comp_env_eq)
+  .
+
+End ProgEquiv.
+
+(** * Forward simulations between two transition semantics. *)
+
+(** The general form of a forward simulation. *)
+
+Module FSIM (Ptr1: Pointer) (Pol1: Policy)
+       (M1: Memory Ptr1 Pol1) (A1: Allocator Ptr1 Pol1 M1)
+       (Ptr2: Pointer) (Pol2: Policy)
+       (M2: Memory Ptr2 Pol2) (A2: Allocator Ptr2 Pol2 M2).
+  Module PE := ProgEquiv Ptr1 Pol1 M1 A1
+                         Ptr2 Pol2 M2 A2.
+  Import PE.
+  Module Csem1 := Csem1.
+  Module S1 := Csem1.Smallstep.
+  Module E1 := S1.Events.
+  Module GV1 := E1.Genv.
+  Module Csem2 := Csem2.
+  Module S2 := Csem2.Smallstep.
+  Module E2 := S2.Events.
+  Module GV2 := E2.Genv.
+  
+  Inductive eventval_match: E1.eventval -> E2.eventval -> Prop :=
+  | MEVint: forall i,
+      eventval_match (E1.EVint i) (E2.EVint i)
+  | MEVlong: forall i,
+      eventval_match (E1.EVlong i) (E2.EVlong i)
+  | MEVfloat: forall f,
+      eventval_match (E1.EVfloat f) (E2.EVfloat f)
+  | MEVsingle: forall f,
+      eventval_match (E1.EVfloat f) (E2.EVfloat f)
+  | MEVptr_global: forall id p1 p2,
+      (Ptr1.concretize p1) = (Ptr2.concretize p2) ->
+      eventval_match (E1.EVptr_global id p1) (E2.EVptr_global id p2)
+  | MEVptr_fun: forall id,
+      eventval_match (E1.EVptr_fun id) (E2.EVptr_fun id)      
+  .
+
+  Inductive ev_list_match: list E1.eventval -> list E2.eventval -> Prop :=
+  | MEVLnil: ev_list_match nil nil
+  | MEVLcons: forall ev1 ev2 evs1 evs2,
+      eventval_match ev1 ev2 ->
+      ev_list_match evs1 evs2 ->
+      ev_list_match (ev1::evs1) (ev2::evs2)
+  .
+  
+  Inductive event_match: E1.event -> E2.event -> Prop :=
+  | MEvent_syscall: forall s evs1 evs2 ev1 ev2,
+      ev_list_match evs1 evs2 ->
+      eventval_match ev1 ev2 ->
+      event_match (E1.Event_syscall s evs1 ev1) (E2.Event_syscall s evs2 ev2)
+  | MEvent_vload: forall chunk id p1 p2 ev1 ev2,
+      (Ptr1.concretize p1) = (Ptr2.concretize p2) ->
+      eventval_match ev1 ev2 ->
+      event_match (E1.Event_vload chunk id p1 ev1) (E2.Event_vload chunk id p2 ev2)
+  | MEvent_vstore: forall chunk id p1 p2 ev1 ev2,
+      (Ptr1.concretize p1) = (Ptr2.concretize p2) ->
+      eventval_match ev1 ev2 ->
+      event_match (E1.Event_vstore chunk id p1 ev1) (E2.Event_vstore chunk id p2 ev2)
+  | MEvent_annot: forall s evs1 evs2,
+      ev_list_match evs1 evs2 ->
+      event_match (E1.Event_annot s evs1) (E2.Event_annot s evs2).
+
+  Inductive match_traces : E1.trace -> E2.trace -> Prop :=
+  | MTnil: match_traces nil nil
+  | MTcons: forall e1 e2 t1 t2,
+      event_match e1 e2 ->
+      match_traces t1 t2 ->
+      match_traces (e1::t1) (e2::t2).
+
+  CoInductive traceinf_match : E1.traceinf -> E2.traceinf -> Prop :=
+  | MEconsinf: forall e1 e2 t1 t2,
+      event_match e1 e2 ->
+      traceinf_match t1 t2 ->
+      traceinf_match (E1.Econsinf e1 t1) (E2.Econsinf e2 t2).
+
+  (** Handy notations, now for both! *)
+
+  Notation " 'S1.Step' L " := (S1.step L (S1.globalenv L) (S1.ce L)) (at level 1) : smallstep_scope.
+  Notation " 'S1.Star' L " := (S1.star (S1.step L) (S1.globalenv L) (S1.ce L)) (at level 1) : smallstep_scope.
+  Notation " 'S1.Plus' L " := (S1.plus (S1.step L) (S1.globalenv L) (S1.ce L)) (at level 1) : smallstep_scope.
+  Notation " 'S1.Forever_silent' L " := (S1.forever_silent (S1.step L) (S1.globalenv L) (S1.ce L)) (at level 1) : smallstep_scope.
+  Notation " 'S1.Forever_reactive' L " := (S1.forever_reactive (S1.step L) (S1.globalenv L) (S1.ce L)) (at level 1) : smallstep_scope.
+  Notation " 'S1.Nostep' L " := (S1.nostep (S1.step L) (S1.globalenv L) (S1.ce L)) (at level 1) : smallstep_scope.
+
+  Notation " 'S2.Step' L " := (S2.step L (S2.globalenv L) (S2.ce L)) (at level 1) : smallstep_scope.
+  Notation " 'S2.Star' L " := (S2.star (S2.step L) (S2.globalenv L) (S2.ce L)) (at level 1) : smallstep_scope.
+  Notation " 'S2.Plus' L " := (S2.plus (S2.step L) (S2.globalenv L) (S2.ce L)) (at level 1) : smallstep_scope.
+  Notation " 'S2.Forever_silent' L " := (S2.forever_silent (S2.step L) (S2.globalenv L) (S2.ce L)) (at level 1) : smallstep_scope.
+  Notation " 'S2.Forever_reactive' L " := (S2.forever_reactive (S2.step L) (S2.globalenv L) (S2.ce L)) (at level 1) : smallstep_scope.
+  Notation " 'S2.Nostep' L " := (S2.nostep (S2.step L) (S2.globalenv L) (S2.ce L)) (at level 1) : smallstep_scope.
+  
+  Open Scope smallstep_scope.
+  
+  Record fsim_properties (L1: S1.semantics) (L2: S2.semantics) (index: Type)
+         (order: index -> index -> Prop)
+         (match_states: index -> S1.state L1 -> S2.state L2 -> Prop) : Prop := {
+      fsim_order_wf: well_founded order;
+      fsim_match_initial_states:
+      forall s1, S1.initial_state L1 s1 ->
+                 exists i, exists s2, S2.initial_state L2 s2 /\ match_states i s1 s2;
+      fsim_match_final_states:
+      forall i s1 s2 r,
+        match_states i s1 s2 -> S1.final_state L1 s1 r -> S2.final_state L2 s2 r;
+      fsim_simulation:
+      forall s1 t1 s1', S1.Step L1 s1 t1 s1' ->
+                       forall i s2, match_states i s1 s2 ->
+                                    exists i', exists s2', exists t2,
+                                      (S2.Plus L2 s2 t2 s2' \/
+                                         (S2.Star L2 s2 t2 s2' /\ order i' i))
+                                      /\ match_states i' s1' s2' /\ match_traces t1 t2;
+      fsim_public_preserved:
+      forall id, GV2.public_symbol L2.(S2.globalenv) id = GV1.public_symbol L1.(S1.globalenv) id
+    }.
+
+Arguments fsim_properties: clear implicits.
+
+Inductive forward_simulation (L1: S1.semantics) (L2: S2.semantics) : Prop :=
+  Forward_simulation (index: Type)
+                     (order: index -> index -> Prop)
+                     (match_states: index -> S1.state L1 -> S2.state L2 -> Prop)
+                     (props: fsim_properties L1 L2 index order match_states).
+
+Arguments Forward_simulation {L1 L2 index} order match_states props.
+
+(** An alternate form of the simulation diagram *)
+
+Lemma fsim_simulation':
+  forall L1 L2 index order match_states, fsim_properties L1 L2 index order match_states ->
+  forall i s1 t1 s1', S1.Step L1 s1 t1 s1' ->
+  forall s2, match_states i s1 s2 ->
+  (exists i', exists s2', exists t2, S2.Plus L2 s2 t2 s2' /\ match_states i' s1' s2' /\ match_traces t1 t2)
+  \/ (exists i', order i' i /\ t1 = E1.E0 /\ match_states i' s1' s2).
+Proof.
+  intros. exploit fsim_simulation; eauto.
+  intros [i' [s2' [t2 [A [B C]]]]]. intuition.
+  left; exists i'; exists s2'; exists t2; auto.
+  inv H3. inv C.
+  right; exists i'; auto.
+  left; exists i'; exists s2'; exists (S2.Events.Eapp t0 t3); split; auto. econstructor; eauto.
+Qed.
+
+(** ** Forward simulation diagrams. *)
+
+(** Various simulation diagrams that imply forward simulation *)
+
+Section FORWARD_SIMU_DIAGRAMS.
+
+  Variable L1: S1.semantics.
+  Variable L2: S2.semantics.
+  
+  Hypothesis public_preserved:
+    forall id, GV2.public_symbol (S2.globalenv L2) id = GV1.public_symbol (S1.globalenv L1) id.
+
+  Variable match_states: S1.state L1 -> S2.state L2 -> Prop.
+
+  Hypothesis match_initial_states:
+    forall s1, S1.initial_state L1 s1 ->
+               exists s2, S2.initial_state L2 s2 /\ match_states s1 s2.
+
+  Hypothesis match_final_states:
+    forall s1 s2 r,
+      match_states s1 s2 ->
+      S1.final_state L1 s1 r ->
+      S2.final_state L2 s2 r.
+
+  (** Simulation when one transition in the first program
+      corresponds to zero, one or several transitions in the second program.
+      However, there is no stuttering: infinitely many transitions
+      in the source program must correspond to infinitely many
+      transitions in the second program. *)
+
+  Section SIMULATION_STAR_WF.
+
+    (** [order] is a well-founded ordering associated with states
+        of the first semantics.  Stuttering steps must correspond
+        to states that decrease w.r.t. [order]. *)
+
+    Variable order: S1.state L1 -> S1.state L1 -> Prop.
+    Hypothesis order_wf: well_founded order.
+
+    Hypothesis simulation:
+      forall s1 t1 s1', S1.Step L1 s1 t1 s1' ->
+                       forall s2, match_states s1 s2 ->
+                                  exists s2' t2,
+                                    (S2.Plus L2 s2 t2 s2' \/ (S2.Star L2 s2 t2 s2' /\ order s1' s1))
+                                    /\ match_states s1' s2' /\ match_traces t1 t2.
+
+    Lemma forward_simulation_star_wf: forward_simulation L1 L2.
+    Proof.
+      apply Forward_simulation with order (fun idx s1 s2 => idx = s1 /\ match_states s1 s2);
+        constructor.
+      - auto.
+      - intros. exploit match_initial_states; eauto. intros [s2 [A B]].
+        exists s1; exists s2; auto.
+      - intros. destruct H. eapply match_final_states; eauto.
+      - intros. destruct H0. subst i. exploit simulation; eauto. intros [s2' [t2 [A [B C]]]].
+        exists s1'; exists s2'; exists t2; intuition auto.
+      - auto.
+    Qed.
+
+  End SIMULATION_STAR_WF.
+
+  Section SIMULATION_STAR.
+
+    (** We now consider the case where we have a nonnegative integer measure
+        associated with states of the first semantics.  It must decrease when we take
+        a stuttering step. *)
+
+    Variable measure: S1.state L1 -> nat.
+
+    Hypothesis simulation:
+      forall s1 t1 s1', S1.Step L1 s1 t1 s1' ->
+                       forall s2, match_states s1 s2 ->
+                                  (exists s2', exists t2, S2.Plus L2 s2 t2 s2' /\ match_states s1' s2' /\ match_traces t1 t2)
+                                  \/ (measure s1' < measure s1 /\ t1 = E1.E0 /\ match_states s1' s2)%nat.
+
+    Lemma forward_simulation_star: forward_simulation L1 L2.
+    Proof.
+      apply forward_simulation_star_wf with (ltof _ measure).
+      apply well_founded_ltof.
+      intros. exploit simulation; eauto. intros [[s2' [t2 [A B]]] | [A [B C]]].
+      exists s2', t2; auto.
+      exists s2, E2.E0; split. right; split. constructor. auto.
+      rewrite B. intuition. constructor.
+    Qed.
+
+  End SIMULATION_STAR.
+
+  (** Simulation when one transition in the first program corresponds
+      to one or several transitions in the second program. *)
+
+  Section SIMULATION_PLUS.
+
+    Hypothesis simulation:
+      forall s1 t1 s1', S1.Step L1 s1 t1 s1' ->
+                       forall s2, match_states s1 s2 ->
+                                  exists s2' t2, S2.Plus L2 s2 t2 s2' /\ match_states s1' s2' /\ match_traces t1 t2.
+
+    Lemma forward_simulation_plus: forward_simulation L1 L2.
+    Proof.
+      apply forward_simulation_star with (measure := fun _ => O).
+      intros. exploit simulation; eauto.
+    Qed.
+
+  End SIMULATION_PLUS.
+
+  (** Lock-step simulation: each transition in the first semantics
+      corresponds to exactly one transition in the second semantics. *)
+  
+  Section SIMULATION_STEP.
+
+    Hypothesis simulation:
+      forall s1 t1 s1', S1.Step L1 s1 t1 s1' ->
+                       forall s2, match_states s1 s2 ->
+                                  exists s2' t2, S2.Step L2 s2 t2 s2' /\ match_states s1' s2' /\ match_traces t1 t2.
+
+    Lemma forward_simulation_step: forward_simulation L1 L2.
+    Proof.
+      apply forward_simulation_plus.
+      intros. exploit simulation; eauto. intros [s2' [t2 [A B]]].
+      exists s2', t2; split; auto. apply S2.plus_one; auto.
+    Qed.
+
+  End SIMULATION_STEP.
+
+  (** Simulation when one transition in the first program
+      corresponds to zero or one transitions in the second program.
+      However, there is no stuttering: infinitely many transitions
+      in the source program must correspond to infinitely many
+      transitions in the second program. *)
+
+  Section SIMULATION_OPT.
+
+    Variable measure: S1.state L1 -> nat.
+
+    Hypothesis simulation:
+      forall s1 t1 s1', S1.Step L1 s1 t1 s1' ->
+                       forall s2, match_states s1 s2 ->
+                                  (exists s2' t2, S2.Step L2 s2 t2 s2' /\ match_states s1' s2' /\ match_traces t1 t2)
+                                  \/ (measure s1' < measure s1 /\ t1 = E1.E0 /\ match_states s1' s2)%nat.
+
+    Lemma forward_simulation_opt: forward_simulation L1 L2.
+    Proof.
+      apply forward_simulation_star with measure.
+      intros. exploit simulation; eauto. intros [[s2' [t2 [A B]]] | [A [B C]]].
+      left; exists s2', t2; split; auto. apply S2.plus_one; auto.
+      right; auto.
+    Qed.
+
+  End SIMULATION_OPT.
+
+End FORWARD_SIMU_DIAGRAMS.
+
+End FSIM. 
